Work in progress

PPermutLib.v
@@ -1,27 +1,28 @@
 Require Export Shared.
-Require Import LibListSorted.
+Require Export PermutLib.
+
 Require Import Setoid.
+Require Import LibListSorted.
 Require Import LibList.
+
+Open Scope permut_scope.
 
 Inductive PPermut: list Context_LF -> list Context_LF -> Prop :=
 | PPermut_nil: PPermut nil nil
 | PPermut_skip: forall G G' w Gamma Gamma', 
-    permut Gamma Gamma' ->
+    Gamma *=* Gamma' ->
     PPermut G G' ->
     PPermut ((w, Gamma)::G) ((w,Gamma')::G')
 | PPermut_swap: forall G w w' Gamma0 Gamma0' Gamma1 Gamma1',
-    permut Gamma0 Gamma1 ->
-    permut Gamma0' Gamma1' ->
+    Gamma0 *=* Gamma1 ->
+    Gamma0' *=* Gamma1' ->
     PPermut ((w, Gamma0) :: (w', Gamma0') :: G)
                 ((w', Gamma1') :: (w, Gamma1) :: G)
 | PPermut_trans: forall G G' G'',
     PPermut G G' -> PPermut G' G'' -> PPermut G G''.
 Hint Constructors PPermut.
 
-Notation "G ~=~ G'" := (PPermut G G') (at level 70) : ppermut_scope. 
-Notation " Ctx *=* Ctx'" := (permut Ctx Ctx') (at level 70) : ppermut_scope.
-
-Open Scope ppermut_scope.
+Notation "G ~=~ G'" := (PPermut G G') (at level 70) : permut_scope. 
 
 Lemma PPermut_reflexive:
   Reflexive PPermut.
@@ -47,8 +48,7 @@ Lemma PPermut_transitive:
   Transitive PPermut.
 exact PPermut_trans.
 Qed.  
-
-Hint Resolve PPermut_reflexive.
+Hint Resolve PPermut_reflexive PPermut_symmetric.
 
 Theorem PPermut'oid: Setoid_Theory _ PPermut.
   split.
@@ -117,15 +117,14 @@ forall G1 G2,
   G1 ++ G2 ~=~ G2 ++ G1.
 induction G1; intros; simpl; rew_app;
 [ auto |
- induction G2]; simpl in *.
-rewrite app_nil_r; auto.
-destruct a; destruct a0;
-transitivity ((v,l) :: (v0, l0) :: G2 ++ G1).
-constructor; auto; apply IHG1.
-transitivity ((v0, l0) :: (v, l) :: G2 ++ G1); auto;
-constructor; auto;
-transitivity ((v,l) :: G1 ++ G2); auto;
-constructor; [ | apply PPermutoid] ; auto.
+ induction G2]; simpl in *;
+[ rewrite app_nil_r; auto |
+  destruct a; destruct a0]; 
+transitivity ((v,l) :: (v0, l0) :: G2 ++ G1);
+[ constructor; auto; apply IHG1 |
+  transitivity ((v0, l0) :: (v, l) :: G2 ++ G1); auto];
+rew_app; constructor; auto;
+transitivity ((v,l) :: G1 ++ G2); auto.
 Qed.
 Hint Resolve PPermut_app_comm.
 
@@ -206,7 +205,7 @@ Lemma PPermut_cons_last_same:
 forall L a,
   a :: L ~=~ L & a.
 induction L; intros;
-[ | rew_app]; auto.
+[ | rew_app]; auto;
 transitivity (a :: a0 :: L); [destruct a0; destruct a | ]; auto.
 Qed.
 
@@ -218,12 +217,14 @@ intros; rewrite H; apply PPermut_cons_last_same.
 Qed.
 Hint Resolve PPermut_cons_last_same PPermut_cons_last.
 
+(* FIXME: Admitted *)
 Lemma PPermut_last_rev_simpl:
 forall G G' a,
   G & a ~=~ G' & a ->
   G ~=~ G'.
 Admitted.
 
+(* FIXME: Admitted *)
 Lemma PPermut_last_rev:
 forall G G' w Gamma Gamma',
   Gamma *=* Gamma' ->
@@ -231,6 +232,7 @@ forall G G' w Gamma Gamma',
   G ~=~ G'.
 Admitted.
 
+(* FIXME: Admitted *)
 Lemma PPermut_split_neq:
 forall G G' w w' Gamma Gamma',
   G & (w, Gamma) ~=~ G' & (w', Gamma') ->
@@ -238,45 +240,60 @@ forall G G' w w' Gamma Gamma',
   exists GH, exists GT, G = GH & (w', Gamma') ++ GT.
 Admitted.
 
+(* FIXME: Admitted *)
 Lemma PPermut_middle_last:
 forall G G' C,
   G ++ G' & C ~=~ G ++ C :: G'.
 Admitted.
 Hint Resolve PPermut_middle_last.
 
+(* FIXME: Admitted *)
+(* FIXME: Too specialized *)
 Lemma PPermut_specialized1:
 forall G G' C C',
   G ++ C :: G' & C' ~=~ G ++ G' ++ C' :: C :: nil.
 Admitted.
 
+(* FIXME: Admitted *)
+(* FIXME: Too specialized *)
 Lemma PPermut_specialized2:
 forall GH GT G Gamma Gamma' Gamma'',
   GH ++ Gamma :: GT & Gamma' ~=~ G & Gamma ->
   GH ++ GT ++ Gamma'' :: Gamma' :: nil ~=~ G & Gamma''.
 Admitted.
 
+(* FIXME: Admitted *)
+(* FIXME: Too specialized *)
 Lemma PPermut_specialized3:
 forall G G' C C',
   G ++ G' ++ C :: C' :: nil ~=~ G ++ C :: G' & C'.
 Admitted.
 
+(* FIXME: Admitted *)
+(* FIXME: Too specialized *)
 Lemma PPermut_specialized4:
 forall G GH GT Gamma Gamma0 Gamma'0,
   GH ++ Gamma :: GT & Gamma'0 ~=~ G & Gamma ->
   G ++ Gamma0 :: Gamma :: nil ~=~ GH ++ GT ++ Gamma0 :: Gamma'0 :: Gamma :: nil.
 Admitted.
 
+(* FIXME: Admitted *)
+(* FIXME: Too specialized *)
 Lemma PPermut_specialized5:
 forall G G' C C' C'',
   G ++ C :: G' ++ C' :: C'' :: nil ~=~ (G ++ G' ++ C' :: C'' :: nil) & C.
 Admitted.
 
+(* FIXME: Admitted *)
+(* FIXME: Too specialized *)
 Lemma PPermut_specialized6:
 forall GH GT C0 C'' C'0,
   GH ++ GT ++ C'0 :: C'' :: C0 :: nil ~=~ GH ++ GT ++ C0 :: C'0 :: C'' :: nil.
 Admitted.
 
-Hint Resolve PPermut_specialized1 PPermut_specialized2 PPermut_specialized3 PPermut_specialized4.
-Hint Resolve PPermut_specialized5 PPermut_specialized6.
-Close Scope ppermut_scope.
+Hint Resolve PPermut_specialized1 PPermut_specialized2 
+             PPermut_specialized3 PPermut_specialized4
+             PPermut_specialized5 PPermut_specialized6.
+
+Close Scope permut_scope.
 
