Shared.v
@@ -1,13 +1,17 @@
-Require Import Metatheory.
+Require Export Utf8.
 
-(* Definitions *)
+(* Package not included in standard Coq builds, needs to be downloaded from
+   http://www.chargueraud.org/softs/ln/ *)
+Require Export Metatheory.
+
+(*** Definitions ***)
 
 (* 
 Types in IS5 system:
    * base type
    * arrow type for functions
-   * box type for universally true terms
-   * diamond type for existentially true terms
+   * box type for universally true terms (= in all the worlds)
+   * diamond type for existentially true terms (= in some of the worlds)
 *)
 Inductive ty :=
 | tvar: ty
@@ -24,6 +28,7 @@ Notation " '<*>' A " := (tdia A)
 
 (*
 Variables for worlds - bound and free
+  We are using locally nameless representation for world variables.
 *)
 Inductive vwo := 
 | bwo: nat -> vwo
@@ -32,20 +37,17 @@ Inductive vwo :=
 
 (*
 Variables for terms - bound and free
+  We are using locally nameless representation for term variables.
 *)
 Inductive vte :=
 | bte: nat -> vte
 | fte: var -> vte
 .
 
-(* Properties *)
+(*** Properties ***)
+
 
 (* Decidability *)
-
-Theorem eq_ty_dec:
-forall a b: ty, {a = b} + {a <> b}.
-  decide equality. 
-Qed.
 
 (* 
 Decidability for var is not expressed in the library, so we need to
@@ -54,19 +56,25 @@ assume is manually.
 Axiom eq_var_dec:
   forall v1 v2: var, {v1 = v2} + {v1 <> v2}.
 
+Theorem eq_ty_dec:
+forall a b: ty, {a = b} + {a <> b}.
+  decide equality. 
+Qed.
+
 Theorem eq_vwo_dec:
 forall w1 w2: vwo, {w1 = w2} + {w1 <> w2}.
-  decide equality.
-  decide equality.
-  apply eq_var_dec.
+  decide equality;
+  [ decide equality |
+    apply eq_var_dec].
 Qed.
 
 Theorem eq_vte_dec:
 forall v1 v2: vte, {v1 = v2} + {v1 <> v2}.
-  decide equality.
-  decide equality.
-  apply eq_var_dec.
+  decide equality;
+  [ decide equality |
+    apply eq_var_dec].
 Qed.
+
 
 (* Free variable extraction *)
 
@@ -82,8 +90,38 @@ match v with
 | bte _ => \{}
 end.
 
-(* Shared definitions *)
+
+(* Calculate shift by one for variable *)
+
+Definition shift_vwo (w: vwo) : vwo :=
+match w with
+  | fwo _ => w
+  | bwo n => bwo (S n)
+end.
+
+Definition shift_vte (v: vte) : vte :=
+match v with
+| fte _ => v
+| bte n => bte (S n)
+end.
+
+
+(* Generating new variable produces fresh variable *)
+
+Lemma generate_fresh:
+forall L w
+  (HIn: w \in L),
+  var_gen L <> w.
+intros;
+intro; subst;
+absurd (var_gen L \in L);
+[apply var_gen_spec | assumption].
+Qed.
+
+
+(*** Shared definitions ***)
+
+(* Potentially removable once we have generic libraries *)
 
 Definition Context_LF := prod var (list (prod var ty)).
 Definition Background_LF := list Context_LF.
-
