label-free/Syntax.v
@@ -1,107 +1,35 @@
 Add LoadPath "./..".
 Require Export Shared.
-Require Export Metatheory.
-Require Import List.
-
-Definition ty_LF := ty.
-
-Inductive ctx_LF :=
-| bctx: nat -> ctx_LF
-| fctx: var -> ctx_LF
-.
-
-Inductive var_LF :=
-| bvar: nat -> var_LF
-| fvar: var -> var_LF
-.
+Require Import LibList.
+Require Import LibListSorted.
 
 Inductive te_LF :=
-| hyp_LF: var_LF -> te_LF
-| lam_LF: ty_LF -> te_LF -> te_LF
+| hyp_LF: vte -> te_LF
+| lam_LF: ty -> te_LF -> te_LF
 | appl_LF: te_LF -> te_LF -> te_LF
 | box_LF: te_LF -> te_LF
-| unbox_fetch_LF: ctx_LF -> te_LF -> te_LF
-| get_here_LF: ctx_LF -> te_LF -> te_LF
-| letdia_get_LF: ctx_LF -> te_LF -> te_LF -> te_LF
+| unbox_fetch_LF: vwo -> te_LF -> te_LF
+| get_here_LF: vwo -> te_LF -> te_LF
+| letdia_get_LF: vwo -> te_LF -> te_LF -> te_LF
 .
 
-Definition var_from_w (w: ctx_LF) :=
-match w with
-| fctx w0 => \{w0}
-| bctx _ => \{}
-end.
 
-Definition var_from_v (v: var_LF) :=
-match v with
-| fvar v0 => \{v0}
-| bvar _ => \{}
-end.
-
-Definition ctx_succ (ctx:ctx_LF) : ctx_LF :=
-match ctx with
-  | fctx _ => ctx
-  | bctx n => bctx (S n)
-end.
-
-Definition var_succ v0 :=
-match v0 with
-| fvar v => fvar v
-| bvar n => bvar (S n)
-end. 
-
-Definition recalc_simpl_ctx (ctx:ctx_LF) : ctx_LF :=
-match ctx with
-    | fctx _ => ctx
-    | bctx n => bctx (S n)
-end.
-
-Definition recalculate_ctx (ctx1: ctx_LF) (ctx2: ctx_LF) : prod ctx_LF ctx_LF :=
-  (recalc_simpl_ctx ctx1, recalc_simpl_ctx ctx2).
-
-
-Definition recalculate_var (v: var_LF) :=
-match v with
-| bvar n => bvar (S n)
-| fvar _ => v
-end.
-
-Axiom eq_var_dec:
-  forall v1 v2: var, {v1 = v2} + {v1 <> v2}.
-
-Theorem eq_context_LF_dec:
-forall c1 c2: Context_LF, {c1 = c2} + {c1 <> c2}.
-intros;
-repeat decide equality;
-apply eq_var_dec.
-Qed.
-
-Require Import LibListSorted.
 (* FIXME: is this going to give us trouble? I.e., should we proove this? *)
 Axiom permut_dec:
-forall (a: list (var * ty_LF)) a',
+forall (a: list (var * ty)) a',
   { permut a a' } + { ~permut a a' }.
+
 
 Theorem permut_context_LF_dec:
 forall (c1 c2: Context_LF),
-  { permut (snd c1) (snd c2) /\ (fst c1) = (fst c2)} + { ~permut (snd c1) (snd c2) \/ (fst c1) <> (fst c2)}.
+  { permut (snd c1) (snd c2) /\ (fst c1) = (fst c2)} + 
+  { ~permut (snd c1) (snd c2) \/ (fst c1) <> (fst c2)}.
 intros; destruct c1 as (w, a); destruct c2 as (w', a');
 destruct (eq_var_dec w w'); subst; simpl;
 destruct (permut_dec a a'); simpl;
 auto.
 Qed.
 
-Theorem eq_var_LF_dec:
-forall v1 v2: var_LF, {v1 = v2} + {v1 <> v2}.
-intros; repeat decide equality;
-apply eq_var_dec.
-Qed.
-
-Theorem eq_ctx_LF_dec:
-forall c1 c2: ctx_LF, {c1 = c2} + {c1 <> c2}.
-intros;
-try repeat decide equality;
-apply eq_var_dec.
-Qed.
 
 (* When a term is context-wise locally closed at level n *)
 Inductive lc_w_n_LF : te_LF -> nat -> Prop :=
@@ -117,19 +45,20 @@ Inductive lc_w_n_LF : te_LF -> nat -> Prop :=
      lc_w_n_LF (box_LF M) n
  | lcw_unbox_fetch_LF: forall M n w,
      lc_w_n_LF M n ->
-     lc_w_n_LF (unbox_fetch_LF (fctx w) M) n
+     lc_w_n_LF (unbox_fetch_LF (fwo w) M) n
  | lcw_get_here_LF: forall M n w ,
      lc_w_n_LF M n ->
-     lc_w_n_LF (get_here_LF (fctx w) M) n
+     lc_w_n_LF (get_here_LF (fwo w) M) n
  | lcw_letdia_get_LF: forall M N n w,
      lc_w_n_LF N (S n) -> lc_w_n_LF M n ->
-     lc_w_n_LF (letdia_get_LF (fctx w) M N) n
+     lc_w_n_LF (letdia_get_LF (fwo w) M N) n
 .
 Definition lc_w_LF (t:te_LF) : Prop := lc_w_n_LF t 0.
 
+
 (* When a term is term-wise locally closed at level n *)
 Inductive lc_t_n_LF: te_LF -> nat -> Prop :=
-| lct_hyp_LF: forall v n, lc_t_n_LF (hyp_LF (fvar v)) n
+| lct_hyp_LF: forall v n, lc_t_n_LF (hyp_LF (fte v)) n
 | lct_lam_LF: forall t M n, 
     lc_t_n_LF M (S n) ->
     lc_t_n_LF (lam_LF t M) n
@@ -141,16 +70,16 @@ Inductive lc_t_n_LF: te_LF -> nat -> Prop :=
      lc_t_n_LF (box_LF M) n
  | lct_unbox_fetch_LF: forall M n w,
      lc_t_n_LF M n ->
-     lc_t_n_LF (unbox_fetch_LF (fctx w) M) n
+     lc_t_n_LF (unbox_fetch_LF (fwo w) M) n
  | lct_get_here_LF: forall M n w ,
      lc_t_n_LF M n ->
-     lc_t_n_LF (get_here_LF (fctx w) M) n
+     lc_t_n_LF (get_here_LF (fwo w) M) n
  | lct_letdia_get_LF: forall M N n w,
      lc_t_n_LF N n -> lc_t_n_LF M n ->
-     lc_t_n_LF (letdia_get_LF (fctx w) M N) n
+     lc_t_n_LF (letdia_get_LF (fwo w) M N) n
 .
-
 Definition lc_t_LF (t:te_LF) : Prop := lc_t_n_LF t 0.
+
 
 (* Calculate list of free worlds used in term M *)
 Fixpoint free_worlds_LF (M: te_LF) : fset var :=
@@ -159,13 +88,14 @@ match M with
 | lam_LF _ M => free_worlds_LF M
 | appl_LF M N => free_worlds_LF M \u free_worlds_LF N
 | box_LF M => free_worlds_LF M
-| unbox_fetch_LF (fctx w) M => \{w} \u free_worlds_LF M
+| unbox_fetch_LF (fwo w) M => \{w} \u free_worlds_LF M
 | unbox_fetch_LF _ M => free_worlds_LF M
-| get_here_LF (fctx w) M => \{w} \u free_worlds_LF M
+| get_here_LF (fwo w) M => \{w} \u free_worlds_LF M
 | get_here_LF _ M => free_worlds_LF M
-| letdia_get_LF (fctx w) M N => \{w} \u free_worlds_LF M \u free_worlds_LF N
+| letdia_get_LF (fwo w) M N => \{w} \u free_worlds_LF M \u free_worlds_LF N
 | letdia_get_LF _ M N => free_worlds_LF M \u free_worlds_LF N
 end.
+
 
 (* Calculate list of unbound worlds of level above n *)
 Fixpoint unbound_worlds (n:nat) (M:te_LF):=
@@ -174,20 +104,21 @@ match M with
 | lam_LF t M => unbound_worlds n M
 | appl_LF M N => unbound_worlds n M ++ unbound_worlds n N
 | box_LF M => unbound_worlds (S n) M
-| unbox_fetch_LF (bctx w) M => w :: unbound_worlds n M
-| unbox_fetch_LF (fctx w) M => unbound_worlds n M
-| get_here_LF (bctx w) M => w :: unbound_worlds n M
-| get_here_LF (fctx w) M => unbound_worlds n M
-| letdia_get_LF (bctx w) M N =>
+| unbox_fetch_LF (bwo w) M => w :: unbound_worlds n M
+| unbox_fetch_LF (fwo w) M => unbound_worlds n M
+| get_here_LF (bwo w) M => w :: unbound_worlds n M
+| get_here_LF (fwo w) M => unbound_worlds n M
+| letdia_get_LF (bwo w) M N =>
   w :: unbound_worlds n M ++ unbound_worlds (S n) N
-| letdia_get_LF (fctx w) M N => unbound_worlds n M ++ unbound_worlds (S n) N
+| letdia_get_LF (fwo w) M N => unbound_worlds n M ++ unbound_worlds (S n) N
 end.
+
 
 (* Calculate list of free variables used in term M *)
 Fixpoint free_vars_LF (M: te_LF) : fset var :=
 match M with
-| hyp_LF (fvar v) => \{v}
-| hyp_LF (bvar _) => \{}
+| hyp_LF (fte v) => \{v}
+| hyp_LF (bte _) => \{}
 | lam_LF _ M => free_vars_LF M
 | appl_LF M N => free_vars_LF M \u free_vars_LF N
 | box_LF M => free_vars_LF M
@@ -196,11 +127,12 @@ match M with
 | letdia_get_LF _ M N => free_vars_LF M \u free_vars_LF N
 end.
 
+
 (* Calculate list of unbound variables of level above n *)
 Fixpoint unbound_vars (n:nat) (M:te_LF):=
 match M with
-| hyp_LF (bvar n) => n::nil
-| hyp_LF (fvar n) => nil 
+| hyp_LF (bte n) => n::nil
+| hyp_LF (fte n) => nil 
 | lam_LF t M => unbound_vars (S n) M
 | appl_LF M N => unbound_vars n M ++ unbound_vars n N
 | box_LF M => unbound_vars n M
@@ -209,17 +141,9 @@ match M with
 | letdia_get_LF _ M N => unbound_vars n M ++ unbound_vars (S n) N
 end.
 
+
 Section Lemmas.
 
-Lemma generate_fresh:
-forall M w
-  (HIn: w \in M),
-  var_gen M <> w.
-intros;
-intro; subst;
-absurd (var_gen M \in M);
-[apply var_gen_spec | assumption].
-Qed.
 
 Lemma closed_w_succ:
 forall M n,
