OkLib.v
@@ -1,0 +1,92 @@
+Require Export Shared.
+Require Export PermutLib.
+Require Export PPermutLib.
+
+Require Import Metatheory.
+Require Import LibList.
+Require Import Setoid.
+
+Open Scope permut_scope.
+
+(*** Definitions ***)
+
+Fixpoint ok A (G: list (var * A)) (Used: list var) : Prop :=
+match G with 
+| nil => True
+| (w, Gamma) :: G => If Mem w Used then False else ok A G (w::Used)
+end.
+
+Definition ok_Bg (G: Background_LF) : Prop :=
+ok (list (var * ty)) G nil  /\
+ok (ty) (flat_map snd G) nil.
+
+Fixpoint used_t_vars (G: Background_LF) :=
+match G with
+| nil => from_list nil
+| (w, Gamma) :: G => from_list (map fst Gamma) \u used_t_vars G
+end. 
+
+Fixpoint used_w_vars (G: Background_LF) :=
+match G with
+| nil => from_list nil
+| (w, Gamma) :: G => \{w} \u used_w_vars G
+end. 
+
+(*** Lemmas ***)
+
+(* FIXME: Admitted *)
+Add Morphism ok_Bg : ok_Bg_PPermut.
+skip.
+Qed.
+
+Lemma ok_Bg_ppermut:
+forall G G',
+  G ~=~ G' ->
+  ok_Bg G ->
+  ok_Bg G'.
+intros; rewrite <- H; auto.
+Qed.
+
+(* FIXME: Admitted *)
+Lemma ok_Bg_permut:
+forall G Ctx Ctx' w,
+  Ctx *=* Ctx' ->
+  ok_Bg ((w, Ctx) :: G) ->
+  ok_Bg ((w, Ctx') :: G).
+Admitted.
+
+(* FIXME: Admitted *)
+Lemma ok_Bg_permut_last:
+forall G Ctx Ctx' w,
+  Ctx *=* Ctx' ->
+  ok_Bg (G ++ (w, Ctx) :: nil) ->
+  ok_Bg (G ++ (w, Ctx') :: nil).
+Admitted.
+
+(* FIXME: Admitted *)
+Lemma ok_Bg_fresh_te:
+forall G Gamma v A w,
+ ok_Bg ((w, Gamma) :: G) ->
+ v \notin (used_t_vars ((w,Gamma)::G)) ->
+ ok_Bg ((w, (v,A)::Gamma) :: G).
+Admitted.
+
+(* FIXME: Admitted *)
+Lemma ok_Bg_fresh_wo:
+forall G w,
+ ok_Bg G ->
+ w \notin (used_w_vars G) ->
+ ok_Bg ((w, nil) :: G).
+Admitted.
+
+(* FIXME: Admitted *)
+Lemma ok_Bg_fresh_wo_te:
+forall G w v A,
+ ok_Bg G ->
+ w \notin (used_w_vars G) ->
+ ok_Bg ((w, (v, A) :: nil) :: G).
+Admitted.
+
+Hint Resolve ok_Bg_fresh_te ok_Bg_fresh_wo ok_Bg_fresh_wo_te.
+
+Close Scope permut_scope.
