PermutLib.v
@@ -1,0 +1,64 @@
+Require Import Setoid.
+Require Export LibListSorted.
+Require Import LibList.
+
+Notation " Ctx *=* Ctx'" := (permut Ctx Ctx') (at level 70) : permut_scope.
+
+Lemma Permut_refl:
+forall (A: Type),
+  Reflexive (@permut A).
+unfold Reflexive; intros; apply permut_refl.
+Qed.
+
+Lemma Permut_sym:
+forall (A: Type),
+  Symmetric (@permut A).
+unfold Symmetric; intros; apply permut_sym; auto.
+Qed.
+
+Lemma Permut_trans:
+forall (A: Type),
+  Transitive (@permut A).
+unfold Transitive; intros; eapply permut_trans; eauto.
+Qed.
+
+Instance Permut_Equivalence A : Equivalence (@permut A) | 10 := {
+  Equivalence_Reflexive := @Permut_refl A ;
+  Equivalence_Symmetric := @Permut_sym A ;
+  Equivalence_Transitive := @Permut_trans A }.
+Hint Resolve Permut_refl Permut_sym.
+
+Open Scope permut_scope.
+
+Lemma test1:
+forall A (G G' G'': list A), G *=* G' -> G'' *=* G' -> G *=* G''.
+intros; rewrite H0; auto.
+Qed.
+
+Add Parametric Morphism A (a:A) : (cons a)
+  with signature @permut A ==> @permut A
+  as Permut_cons.
+auto.
+Qed.
+
+Lemma Permut_last:
+forall (A: Type) (a:A) L L',
+  L *=* L' ->
+  L & a *=* L' & a.
+auto.
+Qed.
+Hint Resolve Permut_cons Permut_last.
+
+Add Parametric Morphism A : (@append A)
+  with signature @permut A ==> @permut A ==> @permut A
+  as Permut_append.
+auto.
+Qed.
+Hint Resolve Permut_append.
+
+(* FIXME: Admitted *)
+Lemma Mem_permut:
+forall A L1 L2, permut L1 L2 -> forall (x : A), Mem x L1 -> Mem x L2.
+Admitted.
+
+Close Scope permut_scope.
