label-free/Substitution.v
@@ -1,20 +1,23 @@
 Add LoadPath "./..".
 Require Export Syntax.
+
+Require Import LibList.
+(*
 Require Import Metatheory.
 Require Import Arith.
-Require Import List.
 
+*)
 Global Reserved Notation " [ M // v ] N " (at level 5).
 Global Reserved Notation " {{ w1 // w2 }} N " (at level 5).
 
 (* Term substitution *)
 
-Fixpoint subst_t (M0: te_LF) (v0: var_LF) (N0: te_LF) :=
+Fixpoint subst_t (M0: te_LF) (v0: vte) (N0: te_LF) :=
 match N0 with
 | hyp_LF v => 
-    if (eq_var_LF_dec v v0) then M0 else N0
+    if (eq_vte_dec v v0) then M0 else N0
 | lam_LF A M => 
-    lam_LF A ([M0 // var_succ v0] M) 
+    lam_LF A ([M0 // shift_vte v0] M) 
 | appl_LF M N => 
     appl_LF ([M0//v0]M) ([M0//v0]N)
 | box_LF M => 
@@ -24,24 +27,24 @@ match N0 with
 | get_here_LF w M =>
     get_here_LF w ([M0//v0]M)
 | letdia_get_LF w M N =>
-    letdia_get_LF w ([M0//v0]M) ([M0//var_succ v0]N)
+    letdia_get_LF w ([M0//v0]M) ([M0//shift_vte v0]N)
 end
 where " [ M // v ] N " := (subst_t M v N) : label_free_is5_scope.
 
-Definition open_var (M: te_LF) (t: te_LF) := subst_t t (bvar 0) M.
+Definition open_var (M: te_LF) (t: te_LF) := subst_t t (bte 0) M.
 Notation " M '^t^' t " := (open_var M t) (at level 5) : label_free_is5_scope.
 
 Open Scope label_free_is5_scope.
 
 (* Context substitution *)
 
-Fixpoint subst_ctx (M0 : te_LF) (ctx1: ctx_LF) (ctx2: ctx_LF) := 
+Fixpoint subst_ctx (M0 : te_LF) (ctx1: vwo) (ctx2: vwo) := 
 match M0 with 
 | hyp_LF n => hyp_LF n
 | lam_LF A M => lam_LF A ({{ctx1//ctx2}}M)
 | appl_LF M N => appl_LF ({{ctx1//ctx2}}M) ({{ctx1//ctx2}}N)
 | box_LF M =>  
-  box_LF ({{ ctx_succ ctx1 // ctx_succ ctx2 }} M)
+  box_LF ({{ shift_vwo ctx1 // shift_vwo ctx2 }} M)
 | unbox_fetch_LF w M =>
   let w' := If w = ctx2 then ctx1 else w in
     unbox_fetch_LF w' ({{ctx1//ctx2}} M)
@@ -50,11 +53,11 @@ match M0 with
     get_here_LF w' ({{ctx1//ctx2}}M)
 | letdia_get_LF w M N =>
   let w' := If w = ctx2 then ctx1 else w in
-    letdia_get_LF w' ({{ctx1//ctx2}} M) ({{ctx_succ ctx1 // ctx_succ ctx2}} N)
+    letdia_get_LF w' ({{ctx1//ctx2}} M) ({{shift_vwo ctx1 // shift_vwo ctx2}} N)
 end
 where " {{ w1 // w2 }} M " := (subst_ctx M w1 w2) : label_free_is5_scope.
 
-Definition open_ctx M ctx := subst_ctx M ctx (bctx 0).
+Definition open_ctx M ctx := subst_ctx M ctx (bwo 0).
 Notation " M ^w^ w  " := (open_ctx M w) (at level 10) : label_free_is5_scope.
 
 
@@ -73,12 +76,12 @@ Qed.
 Lemma no_unbound_vars_LF_subst_var_id:
 forall N M n
   (H_unbound: unbound_vars n N = nil),
-  [M//bvar n] N = N.
+  [M//bte n] N = N.
 induction N; intros; simpl in *;
 try rewrite IHN; auto;
 [ case_if; simpl in *; subst;
   [discriminate | auto] | |];
-apply app_eq_nil in H_unbound;
+apply app_eq_nil_inv in H_unbound;
 destruct H_unbound;
 rewrite IHN1;
 try rewrite IHN2; eauto.
@@ -87,64 +90,99 @@ Qed.
 Lemma no_unbound_worlds_LF_subst_ctx_id_bound:
 forall M n w
   (H_unbound: unbound_worlds n M = nil),
-  {{ w // bctx n }} M = M.
-induction M; intros; simpl in *;
-try (case_if; destruct c; subst; try discriminate);
-try (apply app_eq_nil in H_unbound; destruct H_unbound);
-try rewrite IHM;
-try (rewrite IHM1; try rewrite IHM2);
-eauto.
+  {{ w // bwo n }} M = M.
+induction M; intros; simpl in *.
+reflexivity.
+rewrite IHM; auto.
+rewrite IHM1; try rewrite IHM2; auto. 
+apply app_eq_nil_inv in H_unbound; destruct H_unbound; auto.
+apply app_eq_nil_inv in H_unbound; destruct H_unbound; auto.
+rewrite IHM; auto.
+case_if; subst.
+  inversion H_unbound.
+  rewrite IHM; auto; destruct v; try inversion H_unbound; auto.
+case_if; subst.
+  inversion H_unbound.
+  rewrite IHM; auto; destruct v; try inversion H_unbound; auto.
+case_if; subst.
+  inversion H_unbound.
+  rewrite IHM1; try rewrite IHM2; auto;
+  destruct v. 
+    inversion H_unbound.
+    apply app_eq_nil_inv in H_unbound; destruct H_unbound; auto.
+    inversion H_unbound.
+    apply app_eq_nil_inv in H_unbound; destruct H_unbound; auto.
 Qed.
 
 Lemma no_unbound_worlds_LF_subst_ctx_id_free:
 forall M w w'
   (H_free: w' \notin free_worlds_LF M),
-  {{ w // fctx w' }} M = M.
-induction M; intros; simpl in *;
-try (case_if; destruct c; subst; try discriminate);
-try (rewrite notin_union in H_free; 
-     destruct H_free; rewrite notin_singleton in *);
-try rewrite IHM;
-try (rewrite IHM1; try rewrite IHM2);
-eauto;
-inversion H; subst; elim H0; reflexivity.
+  {{ w // fwo w' }} M = M.
+induction M; intros; simpl in *.
+reflexivity.
+rewrite IHM; auto.
+rewrite IHM1; try rewrite IHM2; auto.
+rewrite IHM; auto.
+case_if; destruct v; subst.
+  discriminate.
+  inversion H; subst;
+  rewrite notin_union in H_free; 
+  destruct H_free; rewrite notin_singleton in *;
+  elim H0; reflexivity.
+  rewrite IHM; auto.
+  rewrite IHM; auto.
+case_if; destruct v; subst.
+  discriminate.
+  inversion H; subst;
+  rewrite notin_union in H_free; 
+  destruct H_free; rewrite notin_singleton in *;
+  elim H0; reflexivity.
+  rewrite IHM; auto.
+  rewrite IHM; auto.
+case_if; destruct v; subst.
+  discriminate.
+  inversion H; subst;
+  rewrite notin_union in H_free; 
+  destruct H_free; rewrite notin_singleton in *;
+  elim H0; reflexivity.
+  rewrite IHM1; try rewrite IHM2; auto.
+  rewrite IHM1; try rewrite IHM2; auto.
 Qed.
 
 Lemma closed_var_subst_var_id:
 forall M n N
   (H_lc: lc_t_n_LF N n),
-  [ M // bvar n ] N = N.
+  [ M // bte n ] N = N.
 intros;
 apply no_unbound_vars_LF_subst_var_id;
 apply closed_t_no_unbound_vars;
 auto.
 Qed.
 
-(* TODO: remove, duplicate *)
+Lemma closed_ctx_subst_ctx_id_free:
+forall M w w'
+  (H_lc: w' \notin free_worlds_LF M),
+  {{w // fwo w'}} M  = M.
+intros;
+apply no_unbound_worlds_LF_subst_ctx_id_free;
+auto.
+Qed.
+
 Lemma closed_ctx_subst_ctx_id_bound:
 forall M w n
   (H_lc: lc_w_n_LF M n),
-  {{w // bctx n}} M  = M.
+  {{w // bwo n}} M  = M.
 intros;
 apply no_unbound_worlds_LF_subst_ctx_id_bound;
 apply closed_w_no_unbound_worlds;
 auto.
 Qed.
 
-Lemma closed_ctx_subst_ctx_id_free:
-forall M w w'
-  (H_lc: w' \notin free_worlds_LF M),
-  {{w // fctx w'}} M  = M.
-intros;
-apply no_unbound_worlds_LF_subst_ctx_id_free;
-auto.
-Qed.
-
 Lemma subst_ctx_comm:
 forall M w w' w'' n
   (Neq: w'' <> w),
-  {{fctx w'//fctx w''}}({{fctx w//bctx n}}M) = 
-  {{fctx w//bctx n}}({{fctx w'//fctx w''}}M).
+  {{fwo w'//fwo w''}}({{fwo w//bwo n}}M) = 
+  {{fwo w//bwo n}}({{fwo w'//fwo w''}}M).
 induction M; intros; simpl;
 repeat case_if; subst; simpl;
 try rewrite IHM;
@@ -156,8 +194,8 @@ Lemma subst_var_comm:
 forall M v v' n N
   (Neq: v <> v')
   (Lc: lc_t_LF N),
-  [ N // fvar v] ([ hyp_LF (fvar v') // bvar n] M) =
-  [hyp_LF (fvar v') // bvar n] ([N // fvar v] M).
+  [ N // fte v] ([ hyp_LF (fte v') // bte n] M) =
+  [hyp_LF (fte v') // bte n] ([N // fte v] M).
 induction M; intros; simpl;
 try (rewrite IHM; auto);
 try (rewrite IHM1; try rewrite IHM2; auto);
@@ -172,41 +210,65 @@ Qed.
 Lemma subst_ctx_id:
 forall M w n
   (HT: w \notin free_worlds_LF M),
-  {{bctx n//fctx w}}({{fctx w//bctx n}}M) = M.
-induction M; intros; simpl in *;
-try (destruct c); repeat case_if;
-try (rewrite notin_union in HT; 
-     rewrite notin_singleton in HT; 
-     destruct HT);
-try (inversion H0; subst);
-try (inversion H; subst);
-try rewrite IHM;
-try (rewrite IHM1; try rewrite IHM2);
-auto;
-elim H1; auto.
+  {{bwo n//fwo w}}({{fwo w//bwo n}}M) = M.
+induction M; intros; simpl in *.
+reflexivity.
+rewrite IHM; auto.
+rewrite IHM1; try rewrite IHM2; auto.
+rewrite IHM; auto.
+repeat case_if; subst.
+  rewrite IHM; auto.
+  rewrite notin_union in HT; 
+  destruct HT; rewrite notin_singleton in *;
+  elim H; reflexivity.
+  destruct v; rewrite IHM; auto.
+repeat case_if; subst.
+  rewrite IHM; auto.
+  rewrite notin_union in HT; 
+  destruct HT; rewrite notin_singleton in *;
+  elim H; reflexivity.
+  destruct v; rewrite IHM; auto.
+repeat case_if; subst.
+  rewrite IHM1; try rewrite IHM2; auto.
+  rewrite notin_union in HT; 
+  destruct HT; rewrite notin_singleton in *;
+  elim H; reflexivity.
+  destruct v; rewrite IHM1; try rewrite IHM2; auto.
 Qed.
 
 Lemma subst_ctx_neutral_free:
 forall M w w' w0
   (HT: w0 \notin free_worlds_LF M),
-  {{w//fctx w0}}({{fctx w0// w'}}M) = {{w//w'}}M.
-induction M; intros; simpl in *;
-try (destruct c); repeat case_if;
-try (rewrite notin_union in HT; 
-     rewrite notin_singleton in HT; 
-     destruct HT);
-try (inversion H0; subst);
-try (inversion H; subst);
-try rewrite IHM;
-try (rewrite IHM1; try rewrite IHM2);
-auto;
-elim H1; auto.
+  {{w//fwo w0}}({{fwo w0// w'}}M) = {{w//w'}}M.
+induction M; intros; simpl in *.
+reflexivity.
+rewrite IHM; auto.
+rewrite IHM1; try rewrite IHM2; auto.
+rewrite IHM; auto.
+repeat case_if; subst.
+  destruct w'; rewrite IHM; auto.
+  rewrite notin_union in HT; 
+  destruct HT; rewrite notin_singleton in *;
+  elim H; reflexivity.
+  destruct v; rewrite IHM; auto.
+repeat case_if; subst.
+  destruct w'; rewrite IHM; auto.
+  rewrite notin_union in HT; 
+  destruct HT; rewrite notin_singleton in *;
+  elim H; reflexivity.
+  destruct v; rewrite IHM; auto.
+repeat case_if; subst.
+  destruct w'; rewrite IHM1; try rewrite IHM2; auto.
+  rewrite notin_union in HT; 
+  destruct HT; rewrite notin_singleton in *;
+  elim H; reflexivity.
+  destruct v; rewrite IHM1; try rewrite IHM2; auto.
 Qed.
 
 Lemma subst_var_neutral_free:
 forall M v n N 
   (HT: v \notin free_vars_LF M),
-  [ N // bvar n] M = [N // fvar v] [hyp_LF (fvar v) // bvar n] M.
+  [ N // bte n] M = [N // fte v] [hyp_LF (fte v) // bte n] M.
 induction M; intros; simpl in *;
 try (rewrite notin_union in HT; destruct HT);
 try erewrite IHM;
@@ -219,41 +281,41 @@ Qed.
 Lemma subst_ctx_neutral_bound:
 forall M w w' n
   (HT: lc_w_n_LF M n),
-  {{w//bctx n}}({{bctx n// w'}}M) = {{w//w'}}M.
+  {{w//bwo n}}({{bwo n// w'}}M) = {{w//w'}}M.
 induction M; intros; simpl in *;
-try (destruct c); repeat case_if;
+try (destruct v); repeat case_if;
 inversion HT; subst;
 try rewrite IHM;
 try (rewrite IHM1; try rewrite IHM2);
 auto.
 Qed.
 
-
 Lemma closed_ctx_step_opening:
 forall M n w
   (HT: lc_w_n_LF M (S n)),
-  lc_w_n_LF ({{fctx w//bctx n}}M) n.
+  lc_w_n_LF ({{fwo w//bwo n}}M) n.
 induction M; intros; inversion HT; subst;
 simpl in *; eauto using lc_w_n_LF;
 case_if; simpl; constructor; eauto.
 Qed.
 
-
 Lemma subst_order_irrelevant_bound:
 forall N w M v m
   (HT_M: lc_w_LF M),
-    [M // v ] ({{w // bctx m}} N)  = 
-    {{w // bctx m}} ([M // v ] N). 
-induction N; intros; simpl in *; unfold var_succ in *;
-try ( (* hyp *)
-  case_if;
+    [M // v ] ({{w // bwo m}} N)  = 
+    {{w // bwo m}} ([M // v ] N). 
+induction N; intros; simpl in *;
+(* hyp *)
+try (case_if;
   [ rewrite closed_ctx_subst_ctx_id_bound |
     simpl]; auto;
   replace m with (0+m) by omega;
   eapply closed_w_addition;
   auto);
-try destruct c; 
-try destruct v;
+unfold shift_vte in *;
+unfold shift_vwo in *;
+destruct v;
+try destruct w;
 try rewrite IHN;
 try (rewrite IHN1; try rewrite IHN2);
 auto.
@@ -262,9 +324,9 @@ Qed.
 Lemma subst_order_irrelevant_free:
 forall N w w' M v
   (HT_M: w' \notin (free_worlds_LF M)),
-    [M // v ] ({{w // fctx w'}} N)  = 
-    {{w // fctx w'}} ([M // v ] N). 
-induction N; intros; simpl in *; unfold var_succ in *;
+    [M // v ] ({{w // fwo w'}} N)  = 
+    {{w // fwo w'}} ([M // v ] N). 
+induction N; intros; simpl in *; unfold shift_vwo in *;
 try ( (* hyp *)
   case_if;
   [ rewrite closed_ctx_subst_ctx_id_free |
@@ -279,15 +341,14 @@ try (rewrite IHN1; try rewrite IHN2);
 auto.
 Qed.
 
-
 Lemma subst_var_preserv_free_worlds:
 forall N v k w,
   w \notin free_worlds_LF N ->
-  w \notin free_worlds_LF [ hyp_LF (fvar v) // bvar k ] N.
+  w \notin free_worlds_LF [ hyp_LF (fte v) // bte k ] N.
 induction N; intros;
 simpl in *;
 repeat case_if;
-try destruct c;
+try destruct v;
 simpl;
 auto.
 Qed.
